Iterator/Consumers/Access.lean
@@ -1,0 +1,31 @@
+/-
+Copyright (c) 2025 Lean FRO, LLC. All rights reserved.
+Released under Apache 2.0 license as described in the file LICENSE.
+Authors: Paul Reichert
+-/
+prelude
+import Iterator.Consumers.Monadic.Access
+import Iterator.Consumers.Partial
+
+@[specialize]
+def Iter.getAtIdx? {α β} [Iterator α Id β] [Productive α Id]
+    (n : Nat) (it : Iter (α := α) β) : Option β :=
+  match it.step with
+  | .yield it' out _ =>
+    match n with
+    | 0 => some out
+    | k + 1 => it'.getAtIdx? k
+  | .skip it' _ => it'.getAtIdx? n
+  | .done _ => none
+termination_by (n, it.finitelyManySkips)
+
+@[specialize]
+partial def Iter.Partial.getAtIdx? {α β} [Iterator α Id β] [Monad Id]
+    (n : Nat) (it : Iter.Partial (α := α) β) : Option β := do
+  match it.it.step with
+  | .yield it' out _ =>
+    match n with
+    | 0 => some out
+    | k + 1 => (⟨it'⟩ : Iter.Partial (α := α) β).getAtIdx? k
+  | .skip it' _ => (⟨it'⟩ : Iter.Partial (α := α) β).getAtIdx? n
+  | .done _ => none
